lots of lemmas/definitions on inf/sup/...

theories/distributions/DistrIneq.ec
@@ -1,12 +1,126 @@
-require import AllCore Distr RealExp RealSeries Ring StdRing StdOrder.
-import RField RealOrder.
-  
-op d : real distr.
-abbrev expr = RealExp.exp.
-abbrev phi t x = expr (t * x)%Real.
-axiom de : forall t, hasE d (phi t).
+require import AllCore Distr RealExp RealSeries Ring StdRing StdOrder DList.
+require import StdBigop.
+import RField RealOrder RealLub Bigreal List.
 
-lemma Chernoff1 (a : real) (t : real) : a >= 0%r => t >= 0%r =>
+abbrev expr = RealExp.exp.
+
+abbrev minus (E:real -> 'a) = (E \o fun x  => 0%r - x).
+
+op glb (E : real -> bool) = - lub (minus E).
+
+op lb (E : real -> bool) (z : real) =
+  forall y, E y => y >= z.
+
+op has_lb  (E : real -> bool) = nonempty (lb E).
+op has_glb (E : real -> bool) = nonempty E /\ has_lb E.
+
+lemma has_lb_ub E : has_lb E <=> has_ub (minus E).
+proof.
+rewrite /has_lb /has_ub.
+split;rewrite /lb /ub /(\o).
++ rewrite /nonempty=> [[]] x lbx. 
++ exists (-x).
++ move=> y //=.
++ rewrite ler_oppr.
++ smt().
+move=>//=.
+rewrite /nonempty=> [[]] x ubx.
+exists (-x).
+move => //=.
+smt().
+qed.
+
+lemma nonempty_minus E : nonempty (minus E) = nonempty E.
+proof.
+smt().
+qed.
+
+lemma has_glb_lub E : has_glb E <=> has_lub (minus E).
+proof.
+by rewrite /has_glb /has_lub has_lb_ub nonempty_minus.
+qed.
+
+lemma glb_upper_bound (E : real -> bool) : has_glb E =>
+  forall x, E x => x >= glb E.
+proof.
+rewrite has_glb_lub=> lub_minusE x Ex.
+by rewrite /glb ler_oppl;apply lub_upper_bound.
+qed.
+
+lemma glb_adherent (E : real -> bool): has_glb E =>
+  forall eps, 0%r < eps => exists e, E e /\ glb E + eps > e.
+proof.
+rewrite has_glb_lub => /lub_adherent eps_adherent eps /eps_adherent.
+move=> [e]; rewrite /(\o); move=> [] E_me;rewrite /lub=> lub_me.
+by exists (-e); split=> //=; rewrite ltr_oppl; smt().
+qed.
+
+op image (f : 'a  -> 'b) x = exists t, x = f t.
+
+lemma image_image (f : real -> real) (g : real -> real) x :
+    image g x => image (f \o g) (f x).
+rewrite /image. smt().
+qed.
+
+lemma lub_min E : nonempty E => (exists m, forall x, E x => m >= x) => has_lub E.
+move => nonempty_E [m] Hm.
+rewrite /has_lub; split=> //=; rewrite /has_ub.
+by exists m.
+qed.
+
+lemma glb_max E : nonempty E => (exists m, forall x, E x => m <= x) => has_glb E.
+proof.
+move => nonemptyE [m] Hm;rewrite /has_glb;split=> //=.
+rewrite /has_lb.
+by exists m.
+qed.
+
+lemma glb_expr (f: real -> real) : has_glb (image (expr \o f)).
+rewrite /has_glb; split=>//=.
++ rewrite /nonempty.
++ exists (expr (f 0%r)). by rewrite /expr_b; exists 0%r.
+rewrite/has_lb /nonempty.
+exists 0%r.
+rewrite /lb /expr_b=> y [] t ->.
+by apply exp_ge0.
+qed.
+
+op inf P (f : real -> real) : real =  glb (fun x => ((image f x) && P x)).
+op sup P (f : real -> real) : real =  lub (fun x => ((image f x) && P x)).
+(*op sup P E : real = lub (fun x => E x && P x).*)
+
+(*lemma inf_opp E P : inf P E = - sup (minus P) (minus E).
+proof.
+rewrite /inf /sup; smt().
+qed.*)
+
+lemma image_minus (f : real -> real) : image f =
+    minus (image (fun x => - (f x))).
+proof.
+rewrite /image /minus /(\o) => //=;smt().
+qed.
+
+lemma inf_opp f P : inf P f = - sup (minus P) (fun x => - (f x)).
+proof.
+rewrite /inf /sup /glb /(\o) => //=.
+by rewrite image_minus.
+qed.
+
+lemma incfun_inf f (g : real -> real) P : (forall x y, x >= y => f x >= f y) =>
+    inf P (f \o g) = f (inf P g).
+move => incf.
+rewrite /inf.
+
+qed.
+
+theory Chernoff.
+
+op d : real distr.
+(*abbrev phi t x = expr (t * x)%Real.*)
+abbrev phi t = E d (fun x => expr (t * x)%Real).
+axiom de : forall t, hasE d (fun x => expr (t * x)%Real).
+
+(*lemma Chernoff1 (a : real) (t : real) : a >= 0%r => t >= 0%r =>
     mu d (fun x => x >= a) <= (expr ( -t * a)) * E d (phi t).
 proof.
 move=> ge0_a ge0_t; rewrite -expZ exp_mu; apply ler_exp_pos => /=.
@@ -15,10 +129,19 @@ move=> x; rewrite b2r_ge0 /(\o) /=; case : (a <= x); last first.
 + move=> _; rewrite -expD; apply exp_ge0.
 move=> le_ax; rewrite -expD -exp0 exp_mono.
 smt().
+qed.*)
+
+lemma Chernoff1 (a : real) (t : real) : a >= 0%r => t >= 0%r =>
+    mu d (fun x => x >= a) <= (expr ( -t * a)) * phi t.
+proof.
+move=> ge0_a ge0_t; rewrite -expZ exp_mu; apply ler_exp_pos => /=.
+apply hasEZ; first by apply de.
+move=> x; rewrite b2r_ge0 /(\o) /=; case : (a <= x); last first.
++ move=> _; rewrite -expD; apply exp_ge0.
+move=> le_ax; rewrite -expD -exp0 exp_mono.
+smt().
 qed.
-
-
-lemma Chernoff2 (a : real) (t : real) : a <= 0%r => t <= 0%r =>
+(*lemma Chernoff2 (a : real) (t : real) : a <= 0%r => t <= 0%r =>
     mu d (fun x => x <= a) <= (expr ( -t * a)) * E d (phi t).
 proof.
 move=> le0_a le0_t; rewrite -expZ exp_mu; apply ler_exp_pos => /=.
@@ -27,4 +150,54 @@ move=> x; rewrite b2r_ge0 /(\o) /=; case : (x <= a); last first.
 + move=> _; rewrite -expD; apply exp_ge0.
 move=> le_xa; rewrite -expD -exp0 exp_mono.
 smt().
+qed.*)
+
+lemma Chernoff2 (a : real) (t : real) : a <= 0%r => t <= 0%r =>
+    mu d (fun x => x <= a) <= (expr ( -t * a)) * phi t.
+proof.
+move=> le0_a le0_t; rewrite -expZ exp_mu; apply ler_exp_pos => /=.
+apply hasEZ; first by apply de.
+move=> x; rewrite b2r_ge0 /(\o) /=; case : (x <= a); last first.
++ move=> _; rewrite -expD; apply exp_ge0.
+move=> le_xa; rewrite -expD -exp0 exp_mono.
+smt().
 qed.
+
+op h (a : real) = sup (fun t => t >= 0%r) (fun t => t * a - ln (phi t)).
+
+lemma Chernoff_inf1 (a : real) : a >= 0%r =>
+    mu d (fun x => x <= a) <= expr (- h a).
+proof.
+move => ge0_a.
+have: expr (- h a) = inf (fun t => t >= 0%r)
+(fun t => expr (- (t * a - ln (phi t)))).
+
+rewrite /h.
+end Chernoff.
+
+theory Additive_Chernoff.
+
+op clamp (r:real) = minr 1%r (maxr 0%r r).
+
+op mBernoulli p = fun x => (b2r (x = 0%r)) * (clamp p) +
+                          (b2r (x = 1%r)) * (1%r - (clamp p)).
+
+op Bernoulli p = Distr.mk (mBernoulli p).
+(* prouver que son esperance est p, ...*)
+
+op n : int.
+op p : real.
+
+axiom gt0_n : 0 < n.
+axiom rg01_p : 0%r <= p <= 1%r.
+
+op X = dlist (Bernoulli p) n.
+
+op e : real.
+axiom gt0_e : e > 0%r.
+
+lemma AddChernoff1 : mu X (fun vs => BRA.big predT idfun vs >=
+                      n%r * (p + e)) <= expr (-2%r * (e^2) * n%r).
+
+
+end Additive_Chernoff.
